src/theory/bir/bir_typing_expSyntax.sig
@@ -3,9 +3,9 @@ sig
    include Abbrev
 
    val type_of_bir_exp_tm   : term
-   val dest_type_of_bir_exp : term -> term * term
+   val dest_type_of_bir_exp : term -> term
    val is_type_of_bir_exp   : term -> bool
-   val mk_type_of_bir_exp   : term * term -> term
+   val mk_type_of_bir_exp   : term -> term
 
    val bir_vars_of_exp_tm   : term
    val dest_bir_vars_of_exp : term -> term
@@ -13,8 +13,8 @@ sig
    val mk_bir_vars_of_exp   : term -> term
 
    val bir_exp_is_well_typed_tm   : term
-   val dest_bir_exp_is_well_typed : term -> term * term
+   val dest_bir_exp_is_well_typed : term -> term
    val is_bir_exp_is_well_typed   : term -> bool
-   val mk_bir_exp_is_well_typed   : term * term -> term
+   val mk_bir_exp_is_well_typed   : term -> term
 
 end
