src/theory/bir-support/bir_exp_congruencesScript.sml
@@ -24,24 +24,24 @@ val _ = new_theory "bir_exp_congruences";
    This is however sufficient for
    simplification. *)
 
-val bir_eval_exp_EQUIV_def = Define `
-  bir_eval_exp_EQUIV e1 e2 <=> (!ext_map env ext_st.
-    (bir_eval_exp ext_map e1 env ext_st = bir_eval_exp ext_map e2 env ext_st))`;
-
+Definition bir_eval_exp_EQUIV_def:
+  bir_eval_exp_EQUIV ext_map e1 e2 = !env ext_st.
+    bir_eval_exp ext_map e1 env ext_st = bir_eval_exp ext_map e2 env ext_st
+End
 
 val bir_eval_exp_EQUIV_IS_EQUIV = store_thm ("bir_eval_exp_EQUIV_IS_EQUIV",
-  ``(!e. bir_eval_exp_EQUIV e e) /\
-    (!e1 e2. bir_eval_exp_EQUIV e1 e2 <=> bir_eval_exp_EQUIV e2 e1) /\
-    (!e1 e2 e3. bir_eval_exp_EQUIV e1 e2 ==> bir_eval_exp_EQUIV e2 e3 ==>
-                bir_eval_exp_EQUIV e1 e3)``,
+  ``(!e. bir_eval_exp_EQUIV ext_map e e) /\
+    (!e1 e2. bir_eval_exp_EQUIV ext_map e1 e2 <=> bir_eval_exp_EQUIV ext_map e2 e1) /\
+    (!e1 e2 e3. bir_eval_exp_EQUIV ext_map e1 e2 ==> bir_eval_exp_EQUIV ext_map e2 e3 ==>
+                bir_eval_exp_EQUIV ext_map e1 e3)``,
 METIS_TAC[bir_eval_exp_EQUIV_def]);
 
 
 (* It is a congruence, it works with substitution *)
 
 val bir_eval_exp_EQUIV_IS_CONG_SUBST = store_thm ("bir_eval_exp_EQUIV_IS_CONG_SUBST",
-``!v ve ve' e. bir_eval_exp_EQUIV ve ve' ==>
-               bir_eval_exp_EQUIV (bir_exp_subst1 v ve e) (bir_exp_subst1 v ve' e)``,
+``!v ve ve' e. bir_eval_exp_EQUIV ext_map ve ve' ==>
+               bir_eval_exp_EQUIV ext_map (bir_exp_subst1 v ve e) (bir_exp_subst1 v ve' e)``,
 
 SIMP_TAC std_ss [bir_eval_exp_EQUIV_def] >>
 METIS_TAC[bir_exp_subst1_EVAL_EQ_GEN]);
@@ -58,147 +58,192 @@ METIS_TAC[bir_exp_subst1_EVAL_EQ_GEN]);
    defined, i.e. only the ones, where all vars are provably initialised and
    we don't get an error message. *)
 
-val bir_exp_CONG_def = Define `bir_exp_CONG e1 e2 <=> (
-    (type_of_bir_exp e1 = type_of_bir_exp e2) /\
-    (bir_vars_of_exp e2 = bir_vars_of_exp e1) /\
-    (!env ty.  bir_env_vars_are_initialised env (bir_vars_of_exp e1) ==>
-               (type_of_bir_exp e1 = SOME ty) ==>
-               (bir_eval_exp e1 env = bir_eval_exp e2 env)))`;
+Definition bir_exp_CONG_def:
+  bir_exp_CONG ext_map e1 e2 <=>
+    type_of_bir_exp e1 = type_of_bir_exp e2 /\
+    bir_vars_of_exp e2 = bir_vars_of_exp e1 /\
+    bir_exts_of_exp e1 = bir_exts_of_exp e2 /\
+    !env ty ext_st.  bir_env_vars_are_initialised env (bir_vars_of_exp e1) /\
+        type_of_bir_exp e1 = SOME ty /\
+        bir_ext_env_exts_are_valid (ext_map,ext_st) (bir_exts_of_exp e1) ==>
+        bir_eval_exp ext_map e1 env ext_st = bir_eval_exp ext_map e2 env ext_st
+End
 
-val bir_exp_CONG_REFL = store_thm ("bir_exp_CONG_REFL",
-  ``!e. bir_exp_CONG e e``,
-SIMP_TAC std_ss [bir_exp_CONG_def]);
+Theorem bir_exp_CONG_REFL:
+  !e ext_map. bir_exp_CONG ext_map e e
+Proof
+  SIMP_TAC std_ss [bir_exp_CONG_def]
+QED
 
+Theorem bir_exp_CONG_TRANS:
+  !e1 e2 e3 ext_map. bir_exp_CONG ext_map e1 e2
+  ==> bir_exp_CONG ext_map e2 e3 ==> bir_exp_CONG ext_map e1 e3
+Proof
+  rw[bir_exp_CONG_def]
+QED
 
-val bir_exp_CONG_TRANS = store_thm ("bir_exp_CONG_TRANS",
-  ``!e1 e2 e3. bir_exp_CONG e1 e2 ==> bir_exp_CONG e2 e3 ==> bir_exp_CONG e1 e3``,
-SIMP_TAC std_ss [bir_exp_CONG_def] >>
-METIS_TAC[]);
+Theorem bir_exp_CONG_SYM:
+  !e1 e2 ext_map. bir_exp_CONG ext_map e1 e2 <=> bir_exp_CONG ext_map e2 e1
+Proof
+  rw[EQ_IMP_THM,bir_exp_CONG_def]
+QED
 
+Theorem bir_exp_CONG_EQUIV_THM:
+  !e1 e2 ext_map. bir_exp_CONG ext_map e1 e2 <=>
+  bir_exp_CONG ext_map e1 = bir_exp_CONG ext_map e2
+Proof
+  fs[FUN_EQ_THM]
+  >> rpt strip_tac >> EQ_TAC
+  >> fs[bir_exp_CONG_def]
+QED
 
-val bir_exp_CONG_SYM = store_thm ("bir_exp_CONG_SYM",
-  ``!e1 e2. bir_exp_CONG e1 e2 <=> bir_exp_CONG e2 e1``,
-SIMP_TAC (std_ss++boolSimps.EQUIV_EXTRACT_ss) [bir_exp_CONG_def] >>
-METIS_TAC[]);
+Theorem bir_exts_of_exp_bir_exp_subst1:
+  !e ve ve' v.
+    bir_vars_of_exp ve = bir_vars_of_exp ve'
+    /\ bir_exts_of_exp ve = bir_exts_of_exp ve' ==>
+  bir_exts_of_exp (bir_exp_subst1 v ve e) =
+  bir_exts_of_exp (bir_exp_subst1 v ve' e)
+Proof
+  Induct
+  >> fs[bir_exp_subst1_REWRS]
+  >> rw[]
+  >> fs[bir_exts_of_exp_def,bir_vars_of_exp_def]
+  >> qmatch_goalsub_rename_tac `bir_exp_subst1 v _ _`
+  >> rpt $ first_x_assum $ drule_all_then $ qspec_then `v` assume_tac
+  >> fs[]
+QED
 
+Theorem bir_ext_env_exts_are_valid_bir_exp_subst1:
+  !e ext_map ext_st v ve.
+  bir_ext_env_exts_are_valid (ext_map,ext_st) (bir_exts_of_exp (bir_exp_subst1 v ve e))
+  ==> bir_ext_env_exts_are_valid (ext_map,ext_st) (bir_exts_of_exp e)
+Proof
+  Induct
+  >> fs[bir_exts_of_exp_def,bir_env_oldTheory.bir_ext_env_exts_are_valid_EMPTY,bir_exp_subst1_REWRS]
+  >> asm_rewrite_tac[]
+  >> rpt strip_tac
+  >> fs[bir_env_oldTheory.bir_ext_env_exts_are_valid_UNION]
+  >> rpt $ first_x_assum drule_all
+  >> fs[]
+QED
 
-val bir_exp_CONG_EQUIV_THM = store_thm ("bir_exp_CONG_EQUIV_THM",
-``!e1 e2. bir_exp_CONG e1 e2 <=> (bir_exp_CONG e1 = bir_exp_CONG e2)``,
+Theorem bir_ext_env_exts_are_valid_bir_exp_subst1':
+  !e ext_map ext_st v ve.
+  v IN bir_vars_of_exp e
+  /\ bir_ext_env_exts_are_valid (ext_map,ext_st) (bir_exts_of_exp (bir_exp_subst1 v ve e))
+  ==> bir_ext_env_exts_are_valid (ext_map,ext_st) (bir_exts_of_exp ve)
+Proof
+  Induct
+  >> fs[bir_exts_of_exp_def,bir_env_oldTheory.bir_ext_env_exts_are_valid_EMPTY,bir_exp_subst1_REWRS,bir_vars_of_exp_def]
+  >> asm_rewrite_tac[]
+  >> rpt strip_tac
+  >> fs[bir_env_oldTheory.bir_ext_env_exts_are_valid_UNION]
+  >> rpt $ first_x_assum drule_all
+  >> fs[]
+QED
 
-SIMP_TAC std_ss [FUN_EQ_THM] >>
-SIMP_TAC std_ss [bir_exp_CONG_def] >>
-METIS_TAC[]);
-
-
-val bir_exp_CONG_IS_CONG_SUBST = store_thm ("bir_exp_CONG_IS_CONG_SUBST",
-``!v ve ve' e. bir_exp_CONG ve ve' ==>
-               bir_exp_CONG (bir_exp_subst1 v ve e) (bir_exp_subst1 v ve' e)``,
-
-REPEAT GEN_TAC >>
-Tactical.REVERSE (Cases_on `v IN bir_vars_of_exp e`) >- (
-  ASM_SIMP_TAC std_ss [bir_exp_subst1_UNUSED_VAR, bir_exp_CONG_REFL]
-) >>
-STRIP_TAC >>
-FULL_SIMP_TAC std_ss [bir_exp_CONG_def, bir_exp_subst1_TYPE_EQ_GEN,
-  bir_exp_subst1_USED_VARS, bir_env_oldTheory.bir_env_vars_are_initialised_UNION] >>
-REPEAT STRIP_TAC >>
-METIS_TAC[bir_exp_subst1_NO_TYPE_SOME, bir_exp_subst1_EVAL_EQ_GEN]);
-
+Theorem bir_exp_CONG_IS_CONG_SUBST:
+  !v ve ve' e ext_map. bir_exp_CONG ext_map ve ve' ==>
+    bir_exp_CONG ext_map (bir_exp_subst1 v ve e) (bir_exp_subst1 v ve' e)
+Proof
+  REPEAT GEN_TAC >>
+  qmatch_goalsub_rename_tac `bir_exp_subst1 v ve e` >>
+  Tactical.REVERSE (Cases_on `v IN bir_vars_of_exp e`) >- (
+    ASM_SIMP_TAC std_ss [bir_exp_subst1_UNUSED_VAR, bir_exp_CONG_REFL]
+  ) >>
+  STRIP_TAC >>
+  fs[bir_exp_CONG_def, bir_exp_subst1_TYPE_EQ_GEN,
+    bir_exp_subst1_USED_VARS, bir_env_oldTheory.bir_env_vars_are_initialised_UNION,
+    bir_exts_of_exp_bir_exp_subst1] >>
+  REPEAT STRIP_TAC >>
+  drule_all_then strip_assume_tac bir_exp_subst1_NO_TYPE_SOME >>
+  drule_all_then assume_tac bir_ext_env_exts_are_valid_bir_exp_subst1 >>
+  drule_all_then assume_tac bir_ext_env_exts_are_valid_bir_exp_subst1' >>
+  irule bir_exp_subst1_EVAL_EQ_GEN >>
+  first_x_assum irule >>
+  fs[]
+QED
 
 (* For practical purposed more insteresting is however a form that can be used
    as congruence rules. *)
 
-val bir_exp_CONG_BASIC_CONG_RULES = store_thm ("bir_exp_CONG_BASIC_CONG_RULES", ``
-(!e e' ty ct.
-      bir_exp_CONG e e' ==>
-      bir_exp_CONG (BExp_Cast ct e ty) (BExp_Cast ct e' ty))
-
-/\
-
-(!e e' et.
-      bir_exp_CONG e e' ==>
-      bir_exp_CONG (BExp_UnaryExp et e) (BExp_UnaryExp et e'))
-
-/\
-
-(!e1 e1' e2 e2' et.
-      bir_exp_CONG e1 e1' ==>
-      bir_exp_CONG e2 e2' ==>
-      bir_exp_CONG (BExp_BinExp et e1 e2) (BExp_BinExp et e1' e2'))
-
-/\
-
-(!e1 e1' e2 e2' et.
-      bir_exp_CONG e1 e1' ==>
-      bir_exp_CONG e2 e2' ==>
-      bir_exp_CONG (BExp_BinPred et e1 e2) (BExp_BinPred et e1' e2'))
-
-/\
-
-(!c c' et et' ef ef'.
-      bir_exp_CONG c c' ==>
-      bir_exp_CONG et et' ==>
-      bir_exp_CONG ef ef' ==>
-      bir_exp_CONG (BExp_IfThenElse c et ef) (BExp_IfThenElse c' et' ef'))
-
-/\
-
-
-(!mem_e mem_e' a_e a_e' en ty.
-      bir_exp_CONG mem_e mem_e' ==>
-      bir_exp_CONG a_e a_e' ==>
-      bir_exp_CONG (BExp_Load mem_e a_e en ty) (BExp_Load mem_e' a_e' en ty))
-
-/\
-
-(!mem_e mem_e' a_e a_e' v_e v_e' en.
-      bir_exp_CONG mem_e mem_e' ==>
-      bir_exp_CONG a_e a_e' ==>
-      bir_exp_CONG v_e v_e' ==>
-      bir_exp_CONG (BExp_Store mem_e a_e en v_e) (BExp_Store mem_e' a_e' en v_e'))
-``,
-
-SIMP_TAC (std_ss++holBACore_ss) [bir_exp_CONG_def,
-  bir_env_oldTheory.bir_env_vars_are_initialised_UNION, type_of_bir_exp_def] >>
-REPEAT STRIP_TAC >> ASM_SIMP_TAC std_ss []);
+Theorem bir_exp_CONG_BASIC_CONG_RULES:
+  (!e e' ty ct ext_map.
+      bir_exp_CONG ext_map e e' ==>
+      bir_exp_CONG ext_map (BExp_Cast ct e ty) (BExp_Cast ct e' ty)) /\
+  (!e e' et ext_map.
+      bir_exp_CONG ext_map e e' ==>
+      bir_exp_CONG ext_map (BExp_UnaryExp et e) (BExp_UnaryExp et e')) /\
+  (!e1 e1' e2 e2' et ext_map.
+      bir_exp_CONG ext_map e1 e1' ==>
+      bir_exp_CONG ext_map e2 e2' ==>
+      bir_exp_CONG ext_map (BExp_BinExp et e1 e2) (BExp_BinExp et e1' e2')) /\
+  (!e1 e1' e2 e2' et ext_map.
+      bir_exp_CONG ext_map e1 e1' ==>
+      bir_exp_CONG ext_map e2 e2' ==>
+      bir_exp_CONG ext_map (BExp_BinPred et e1 e2) (BExp_BinPred et e1' e2')) /\
+  (!c c' et et' ef ef' ext_map.
+      bir_exp_CONG ext_map c c' ==>
+      bir_exp_CONG ext_map et et' ==>
+      bir_exp_CONG ext_map ef ef' ==>
+      bir_exp_CONG ext_map (BExp_IfThenElse c et ef) (BExp_IfThenElse c' et' ef')) /\
+  (!ext_map ext ty.
+      bir_exp_CONG ext_map (BExp_ExtGet ext ty) (BExp_ExtGet ext ty)) /\
+  (!mem_e mem_e' a_e a_e' en ty ext_map.
+      bir_exp_CONG ext_map mem_e mem_e' ==>
+      bir_exp_CONG ext_map a_e a_e' ==>
+      bir_exp_CONG ext_map (BExp_Load mem_e a_e en ty) (BExp_Load mem_e' a_e' en ty)) /\
+  (!mem_e mem_e' a_e a_e' v_e v_e' en ext_map.
+      bir_exp_CONG ext_map mem_e mem_e' ==>
+      bir_exp_CONG ext_map a_e a_e' ==>
+      bir_exp_CONG ext_map v_e v_e' ==>
+      bir_exp_CONG ext_map (BExp_Store mem_e a_e en v_e) (BExp_Store mem_e' a_e' en v_e'))
+Proof
+  SIMP_TAC (std_ss++holBACore_ss) [bir_exp_CONG_def,
+    bir_env_oldTheory.bir_env_vars_are_initialised_UNION, type_of_bir_exp_def] >>
+  REPEAT STRIP_TAC >> ASM_SIMP_TAC std_ss [] >>
+  simp[Once FUN_EQ_THM,bir_eval_exp_def]
+QED
 
 
 (* Now real simplifications.
    TODO: Add Many more! *)
 
-val bir_exp_CONG_simp_IDEMPOTENT_AND = store_thm ("bir_exp_CONG_simp_IDEMPOTENT_AND",
-   ``!e.
-     (?ty. bir_type_is_Imm ty /\ (type_of_bir_exp e = SOME ty)) ==>
-     bir_exp_CONG (BExp_BinExp BIExp_And e e) e``,
-
-REPEAT STRIP_TAC >>
-ASM_SIMP_TAC std_ss [bir_exp_CONG_def, bir_vars_of_exp_def,
-  UNION_IDEMPOT, type_of_bir_exp_def, pairTheory.pair_case_thm,
-  bir_eval_exp_def] >>
-REPEAT STRIP_TAC >>
-Cases_on `bir_eval_exp e env` >- (
-  FULL_SIMP_TAC (std_ss++holBACore_ss) [bir_eval_bin_exp_def]
-) >>
-subgoal `ty = type_of_bir_val x` >- (
-  IMP_RES_TAC type_of_bir_exp_THM_with_init_vars >>
-  `x = va` by FULL_SIMP_TAC (std_ss++holBACore_ss) [] >>
-  FULL_SIMP_TAC (std_ss++holBACore_ss) []
-) >>
-Cases_on `x` >> (
-  FULL_SIMP_TAC (std_ss++holBACore_ss) [bir_eval_bin_exp_def]
-) >>
-rename1 `bir_bin_exp _ v v = v` >>
-Cases_on `v` >> (
-  SIMP_TAC (std_ss++holBACore_ss) [wordsTheory.WORD_AND_IDEM]
-)
-);
+Theorem bir_exp_CONG_simp_IDEMPOTENT_AND:
+  !e ext_map ty.
+     bir_type_is_Imm ty /\ type_of_bir_exp e = SOME ty ==>
+     bir_exp_CONG ext_map (BExp_BinExp BIExp_And e e) e
+Proof
+  REPEAT STRIP_TAC >>
+  ASM_SIMP_TAC std_ss [bir_exp_CONG_def, bir_vars_of_exp_def,
+    UNION_IDEMPOT, type_of_bir_exp_def, pairTheory.pair_case_thm,
+    bir_eval_exp_def,FUN_EQ_THM] >>
+  REPEAT STRIP_TAC >>
+  qmatch_goalsub_rename_tac `_ = bir_eval_exp ext_map e env x` >>
+  Cases_on `bir_eval_exp ext_map e env x` >- (
+    FULL_SIMP_TAC (std_ss++holBACore_ss) [bir_eval_bin_exp_def]
+  ) >>
+  qmatch_goalsub_rename_tac `SOME x'` >>
+  subgoal `ty = type_of_bir_val x'` >- (
+    IMP_RES_TAC type_of_bir_exp_THM_with_init_vars >>
+    `x' = va` by FULL_SIMP_TAC (std_ss++holBACore_ss) [] >>
+    FULL_SIMP_TAC (std_ss++holBACore_ss) []
+  ) >>
+  Cases_on `x` >> (
+    FULL_SIMP_TAC (std_ss++holBACore_ss) [bir_eval_bin_exp_def]
+  ) >>
+  rename1 `bir_bin_exp _ v v = v` >>
+  Cases_on `v` >> (
+    SIMP_TAC (std_ss++holBACore_ss) [wordsTheory.WORD_AND_IDEM]
+  )
+QED
 
 
 
 val bir_exp_CONG_simp_IDEMPOTENT_OR = store_thm ("bir_exp_CONG_simp_IDEMPOTENT_OR",
-   ``!e.
+   ``!e ext_map.
      (?ty. bir_type_is_Imm ty /\ (type_of_bir_exp e = SOME ty)) ==>
-     bir_exp_CONG (BExp_BinExp BIExp_Or e e) e``,
+     bir_exp_CONG ext_map (BExp_BinExp BIExp_Or e e) e``,
 
 
 REPEAT STRIP_TAC >>
@@ -243,7 +288,7 @@ val bir_exp_CONG_WEAK_def = Define `bir_exp_CONG_WEAK e1 e2 <=> (
                (bir_eval_exp e1 env = bir_eval_exp e2 env)))`;
 
 val bir_exp_CONG_WEAK_IS_WEAK = store_thm ("bir_exp_CONG_WEAK_IS_WEAK",
- ``!e1 e2. bir_exp_CONG e1 e2 ==> bir_exp_CONG_WEAK e1 e2``,
+ ``!e1 e2. bir_exp_CONG ext_map e1 e2 ==> bir_exp_CONG_WEAK e1 e2``,
 SIMP_TAC std_ss [bir_exp_CONG_def, bir_exp_CONG_WEAK_def, SUBSET_REFL]);
 
 val bir_exp_CONG_WEAK_REFL = store_thm ("bir_exp_CONG_WEAK_REFL",
